make `invariant` opaque

src/cddl/pulse/CDDL.Pulse.Serialize.Gen.MapGroup.ZeroOrMore.Aux2.Invariant.fsti
@@ -174,7 +174,7 @@ let impl_serialize_map_zero_or_more_iterator_gen_invariant1
   impl_serialize_map_zero_or_more_iterator_gen_invariant_min p sp1 sp2 except min v0 v /\
   impl_serialize_map_zero_or_more_iterator_gen_invariant_max p sp1 sp2 except max v0 v 
 
-assume val impl_serialize_map_zero_or_more_iterator_gen_invariant
+let impl_serialize_map_zero_or_more_iterator_gen_invariant2
   (#pe: cbor_parser)
   (#minl: (cbor_min_length pe))
   (#maxl: (cbor_max_length pe))
@@ -197,3 +197,55 @@ assume val impl_serialize_map_zero_or_more_iterator_gen_invariant
   (max: option nat)
   (res: bool)
 : prop
+= admit ()
+
+val impl_serialize_map_zero_or_more_iterator_gen_invariant
+  (#pe: cbor_parser)
+  (#minl: (cbor_min_length pe))
+  (#maxl: (cbor_max_length pe))
+  (p: (cbor_map_parser minl maxl))
+  (#key: typ) (#tkey: Type0)
+  (sp1: (spec key tkey true))
+  (#value: typ) (#tvalue: Type0)
+  (#inj: bool)
+  (sp2: (spec value tvalue inj))
+  (except: map_constraint { inj \/ map_constraint_value_injective key sp2.parser except })
+  (em: bool)
+  (out: S.slice U8.t)
+  (vout: Seq.seq U8.t)
+  (size: SZ.t)
+  (count: U64.t)
+  (m: cbor_map)
+  (v0: Map.t tkey (list tvalue))
+  (v: Map.t tkey (list tvalue))
+  (min: nat)
+  (max: option nat)
+  (res: bool)
+: prop
+
+val impl_serialize_map_zero_or_more_iterator_gen_invariant_reveal
+  (#pe: cbor_parser)
+  (#minl: (cbor_min_length pe))
+  (#maxl: (cbor_max_length pe))
+  (p: (cbor_map_parser minl maxl))
+  (#key: typ) (#tkey: Type0)
+  (sp1: (spec key tkey true))
+  (#value: typ) (#tvalue: Type0)
+  (#inj: bool)
+  (sp2: (spec value tvalue inj))
+  (except: map_constraint { inj \/ map_constraint_value_injective key sp2.parser except })
+  (em: bool)
+  (out: S.slice U8.t)
+  (vout: Seq.seq U8.t)
+  (size: SZ.t)
+  (count: U64.t)
+  (m: cbor_map)
+  (v0: Map.t tkey (list tvalue))
+  (v: Map.t tkey (list tvalue))
+  (min: nat)
+  (max: option nat)
+  (res: bool)
+: Lemma
+  (impl_serialize_map_zero_or_more_iterator_gen_invariant p sp1 sp2 except em out vout size count m v0 v min max res <==>
+    impl_serialize_map_zero_or_more_iterator_gen_invariant2 p sp1 sp2 except em out vout size count m v0 v min max res
+  )
